examples/dsls/mini_steel/Pulse.Checker.Inference.fsti
@@ -1,14 +1,17 @@
 module Pulse.Checker.Inference
 
 open Pulse.Syntax
+open Pulse.Typing
 
 module T = FStar.Tactics
+module R = FStar.Reflection
 
-val try_inst_uvs_in_goal (ctxt:term)
+val try_inst_uvs_in_goal (f:R.env) (g:env)
+                         (ctxt:term)
                          (goal:vprop)
   : T.Tac (list (term & term))
 
-val infer (head:term) (t_head:term) (ctxt_pre:term)
+val infer (f:R.env) (g:env) (head:term) (t_head:term) (ctxt_pre:term)
   : T.Tac st_term
 
 val apply_solution (sol:list (term & term)) (t:term)
@@ -17,5 +20,15 @@ val apply_solution (sol:list (term & term)) (t:term)
 val contains_uvar (t:term)
   : bool
 
-val try_unify (l r:term)
+val try_unify (f:R.env) (g:env) (l r:term)
   : T.Tac (list (term & term))
+
+
+
+
+
+
+
+
+
+
