src/tactics/FStar.Tactics.Types.fsti
@@ -25,6 +25,8 @@ module Range = FStar.Compiler.Range
 module BU = FStar.Compiler.Util
 module O = FStar.Options
 
+module Core = FStar.TypeChecker.Core
+
 (*
    f: x:int -> P
    ==================
@@ -115,3 +117,9 @@ val check_goal_solved' : goal -> option term
 val check_goal_solved  : goal -> bool
 val get_phi            : goal -> option term
 val is_irrelevant      : goal -> bool
+
+type unfold_side =
+  | Left
+  | Right
+  | Both
+  | Neither
