ulib/FStar.Tactics.Util.fst
@@ -106,3 +106,12 @@ let rec tryFind (#a:Type) (f:a -> Tac bool) (l:list a) : Tac bool =
   | hd::tl ->
     if f hd then true
     else tryFind f tl
+
+let rec fold_left2 (#a #b #c:Type) (f:a -> b -> c -> Tac a) (x:a) (l1:list b) (l2:list c)
+  : TacH a
+      (requires fun _ -> length l1 == length l2)
+      (ensures fun _ _ -> True) =
+  match l1, l2 with
+  | [], [] -> x
+  | hd1::tl1, hd2::tl2 ->
+    fold_left2 f (f x hd1 hd2) tl1 tl2
